Fix bin/build -t1

examples/Crypto/RSA/congruentScript.sml
@@ -15,22 +15,22 @@ quietdec := false;
 
 val ARW = RW_TAC arith_ss;
 
-Definition CONGRUENT:   congruent a b n = ?c d. a+c*n = b+d*n
+Definition congruent_def:   congruent a b n = ?c d. a+c*n = b+d*n
 End
 
 
 val CONGRUENT_REF = store_thm("CONGRUENT_REF",
                         Term `!a n. congruent a a n`,
-                        PROVE_TAC[CONGRUENT]);
+                        PROVE_TAC[congruent_def]);
 
 val CONGRUENT_SYM = store_thm("CONGRUENT_SYM",
                         Term `!a b n. congruent a b n = congruent b a n`,
-                        PROVE_TAC[CONGRUENT]);
+                        PROVE_TAC[congruent_def]);
 
 val CONGRUENT_TRANS = store_thm("CONGRUENT_TRANS",
                         Term `!a b c n. congruent a b n /\ congruent b c n
                                 ==> congruent a c n`,
-                        ARW[CONGRUENT]
+                        ARW[congruent_def]
                         THEN EXISTS_TAC (Term `c'+c''`)
                         THEN EXISTS_TAC (Term `d+d'`)
                         THEN ARW[RIGHT_ADD_DISTRIB]
@@ -38,7 +38,7 @@ val CONGRUENT_TRANS = store_thm("CONGRUENT_TRANS",
 
 val CONGRUENT_MULT_0 = store_thm("CONGRUENT_MULT_0",
                         Term `!a b n. congruent a 0 n ==> congruent (a*b) 0 n`,
-                        ARW[CONGRUENT]
+                        ARW[congruent_def]
                         THEN EXISTS_TAC (Term `b*c`)
                         THEN EXISTS_TAC (Term `b*d`)
                         THEN PROVE_TAC[RIGHT_ADD_DISTRIB,MULT_ASSOC,MULT_SYM]);
@@ -46,7 +46,7 @@ val CONGRUENT_MULT_0 = store_thm("CONGRUENT_MULT_0",
 val CONGRUENT_ADD = store_thm("CONGRUENT_ADD",
                         Term `!a b c d n. congruent a b n /\ congruent c d n
                                  ==> congruent (a+c) (b+d) n`,
-                        ARW[CONGRUENT]
+                        ARW[congruent_def]
                         THEN EXISTS_TAC (Term `c'+c''`)
                         THEN EXISTS_TAC (Term `d'+d''`)
                         THEN ARW[RIGHT_ADD_DISTRIB]);
@@ -56,7 +56,7 @@ val CONGRUENT_TIMES = store_thm("CONGRUENT_TIMES",
                         Term `!a b c n. congruent a b n
                                          ==>
                                         congruent (a*c) (b*c) n`,
-                        ARW[CONGRUENT]
+                        ARW[congruent_def]
                         THEN EXISTS_TAC (Term `c'*c`)
                         THEN EXISTS_TAC (Term `d*c`)
                         THEN  ARW[RIGHT_ADD_DISTRIB]
@@ -69,7 +69,7 @@ val CONGRUENT_MULT = store_thm("CONGRUENT_MULT",
                         Term `!a b c d n. congruent a b n /\ congruent c d n
                                             ==>
                                           congruent (a*c) (b*d) n`,
-                        ARW[CONGRUENT]
+                        ARW[congruent_def]
                         THEN EXISTS_TAC (Term `a*c''+c*c'+c'*c''*n`)
                         THEN EXISTS_TAC (Term `b*d''+d*d'+d'*d''*n`)
                         THEN `(a * c + (a * c'' + c * c' + c' * c'' * n) * n)
@@ -94,13 +94,13 @@ val CONGRUENT_LE_EX = store_thm("CONGRUENT_LE_EX",
                         Term `!a b n. b <= a /\ congruent a b n
                                           ==>
                                       ?c. a = b + c*n`,
-                        ARW[CONGRUENT]
+                        ARW[congruent_def]
                         THEN EXISTS_TAC (Term `d-c`)
                         THEN ARW[RIGHT_SUB_DISTRIB]
                      );
 val CONGRUENT_LE_1 = store_thm("CONGRUENT_LE_1",
                         Term `!a n. 1 < n /\ congruent a 1 n ==> 1 <= a`,
-                        Cases_on `a` THEN ARW[CONGRUENT]
+                        Cases_on `a` THEN ARW[congruent_def]
                         THEN SPOSE_NOT_THEN STRIP_ASSUME_TAC
                         THEN `(c-d)*n = 1`
                           by (ASM_REWRITE_TAC[RIGHT_SUB_DISTRIB] THEN ARW[])
@@ -112,11 +112,11 @@ val DIVIDES_CONGRUENT = store_thm("DIVIDES_CONGRUENT",
                         Term `!a n. divides n a = congruent a 0 n`,
                         ARW[] THEN
                         `divides n a ==> congruent a 0 n`
-                          by (ARW[divides_def,CONGRUENT]
+                          by (ARW[divides_def,congruent_def]
                                THEN EXISTS_TAC (Term `0`)
                                THEN EXISTS_TAC (Term`q:num`) THEN ARW[]) THEN
                         `congruent a 0 n ==> divides n a`
-                          by (ARW[divides_def,CONGRUENT]
+                          by (ARW[divides_def,congruent_def]
                                THEN EXISTS_TAC (Term `d-c`) THEN ARW[]) THEN
                         PROVE_TAC[]
                      );
@@ -129,4 +129,3 @@ val CONGRUENT_DIVIDES = store_thm("CONGRUENT_DIVIDES",
                          THEN ARW[DIVIDES_MULT,ADD_SUB]
                          THEN PROVE_TAC[DIVIDES_MULT,ADD_SUB,
                                         DIVIDES_REFL,MULT_SYM]);
-
