examples/arm/v7/arm_opsemScript.sml
@@ -866,7 +866,7 @@ End
 
 (* ------------------------------------------------------------------------ *)
 
-Definition null_check_if_thumbee_def:
+Definition null_check_if_thumbEE_def:
   null_check_if_thumbEE ii n (f:unit M) =
     current_instr_set ii >>=
     (\iset.
@@ -4003,4 +4003,3 @@ val _ = List.app
             (map fst (List.drop (instructions,2)))
 
 (* ------------------------------------------------------------------------ *)
-
